src/cbor/pulse/raw/CBOR.Pulse.Raw.Format.Nondet.Compare.fsti
@@ -1,0 +1,71 @@
+module CBOR.Pulse.Raw.Format.Nondet.Compare
+include CBOR.Spec.Raw.Format
+include CBOR.Spec.Raw.Valid
+include CBOR.Pulse.Raw.Match
+open Pulse.Lib.Pervasives
+
+val cbor_match_equal_serialized_tagged
+  (c1 c2: cbor_serialized)
+  (#pm1: perm)
+  (#r1: Ghost.erased raw_data_item { Tagged? r1 })
+  (#pm2: perm)
+  (#r2: Ghost.erased raw_data_item { Tagged? r2 })
+: stt bool
+  (cbor_match_serialized_tagged c1 pm1 r1 **
+    cbor_match_serialized_tagged c2 pm2 r2 **
+    pure (Tagged?.tag r1 == Tagged?.tag r2 /\
+      valid_raw_data_item r1 /\
+      valid_raw_data_item r2
+    ) 
+  )
+  (fun res ->
+    cbor_match_serialized_tagged c1 pm1 r1 **
+    cbor_match_serialized_tagged c2 pm2 r2 **
+    pure (
+      res == raw_equiv r1 r2
+    )
+  )
+
+val cbor_match_compare_serialized_array
+  (c1 c2: cbor_serialized)
+  (#pm1: perm)
+  (#r1: Ghost.erased raw_data_item { Array? r1 })
+  (#pm2: perm)
+  (#r2: Ghost.erased raw_data_item { Array? r2 })
+: stt bool
+  (cbor_match_serialized_array c1 pm1 r1 **
+    cbor_match_serialized_array c2 pm2 r2 **
+    pure (Array?.len r1 == Array?.len r2 /\
+      valid_raw_data_item r1 /\
+      valid_raw_data_item r2
+    )
+  )
+  (fun res ->
+    cbor_match_serialized_array c1 pm1 r1 **
+    cbor_match_serialized_array c2 pm2 r2 **
+    pure (
+      res == raw_equiv r1 r2
+    )
+  )
+
+val cbor_match_compare_serialized_map
+  (c1 c2: cbor_serialized)
+  (#pm1: perm)
+  (#r1: Ghost.erased raw_data_item { Map? r1 })
+  (#pm2: perm)
+  (#r2: Ghost.erased raw_data_item { Map? r2 })
+: stt bool
+  (cbor_match_serialized_map c1 pm1 r1 **
+    cbor_match_serialized_map c2 pm2 r2 **
+    pure (Map?.len r1 == Map?.len r2 /\
+      valid_raw_data_item r1 /\
+      valid_raw_data_item r2
+    )
+  )
+  (fun res ->
+    cbor_match_serialized_map c1 pm1 r1 **
+    cbor_match_serialized_map c2 pm2 r2 **
+    pure (
+      res == raw_equiv r1 r2
+    )
+  )
